pure spec

OpenvmFv/Spec/Load/lw.lean
@@ -31,6 +31,13 @@ namespace PureSpec
     nextPC : BitVec 32
     rd : Option (Finset.Icc 1 31 × BitVec 32)
 
+  private lemma range (bv : BitVec 5) (h : bv ≠ 0)
+  : bv.toNat ∈ Finset.Icc 1 31
+  := by
+    apply Finset.mem_Icc.mpr
+    obtain ⟨x: Fin 32⟩ := bv
+    fin_cases x <;> simp_all
+
   def execute_LOAD_lw_pure (input : LwInput) : LwOutput := {
     nextPC := input.PC + 4#32
     rd := if h: input.rd = 0
@@ -38,16 +45,15 @@ namespace PureSpec
       else .some (
         ⟨
           input.rd.toNat,
-          by
-            apply Finset.mem_Icc.mpr;
-            done
+          range input.rd h
         ⟩,
         input.data3 ++ input.data2 ++ input.data1 ++ input.data0
       )
     : LwOutput
   }
 
-  def bitvec_to_reg (bv: BitVec 5) : Register :=
+  -- just used to allow the same tactics to handle the case for each non-zero register
+  private def bitvec_to_reg (bv: BitVec 5) : Register :=
     match bv with
       | 0#5 => Register.x1 -- purely used for totality, does not come up
       | 1#5 => Register.x1
@@ -114,6 +120,291 @@ namespace PureSpec
     i.r1_val.toNat + (BitVec.signExtend 32 i.imm).toNat + 4 < 2^32
 
   set_option maxHeartbeats 0 in
+  lemma r1_of_write_state
+    {r1 : BitVec 5}
+    {r1_val : BitVec 32}
+    (pc : BitVec 32)
+    (h_r1_val : LeanRV32D.Functions.rX_bits (regidx.Regidx r1) state = EStateM.Result.ok r1_val state)
+  :
+    LeanRV32D.Functions.rX_bits (regidx.Regidx r1) (write_reg_state state Register.nextPC (Sail.BitVec.addInt pc 4)) =
+    EStateM.Result.ok r1_val (write_reg_state state Register.nextPC (Sail.BitVec.addInt pc 4))
+  := by
+    by_cases h_r1: r1 = 0
+    . simp [
+        h_r1, LeanRV32D.Functions.rX_bits, LeanRV32D.Functions.rX
+      ] at ⊢ h_r1_val
+      exact h_r1_val
+    by_cases h_r1 : r1 = 1 <;> [
+      skip ; by_cases h_r1 : r1 = 2 <;> [
+      skip ; by_cases h_r1 : r1 = 3 <;> [
+      skip ; by_cases h_r1 : r1 = 4 <;> [
+      skip ; by_cases h_r1 : r1 = 5 <;> [
+      skip ; by_cases h_r1 : r1 = 6 <;> [
+      skip ; by_cases h_r1 : r1 = 7 <;> [
+      skip ; by_cases h_r1 : r1 = 8 <;> [
+      skip ; by_cases h_r1 : r1 = 9 <;> [
+      skip ; by_cases h_r1 : r1 = 10 <;> [
+      skip ; by_cases h_r1 : r1 = 11 <;> [
+      skip ; by_cases h_r1 : r1 = 12 <;> [
+      skip ; by_cases h_r1 : r1 = 13 <;> [
+      skip ; by_cases h_r1 : r1 = 14 <;> [
+      skip ; by_cases h_r1 : r1 = 15 <;> [
+      skip ; by_cases h_r1 : r1 = 16 <;> [
+      skip ; by_cases h_r1 : r1 = 17 <;> [
+      skip ; by_cases h_r1 : r1 = 18 <;> [
+      skip ; by_cases h_r1 : r1 = 19 <;> [
+      skip ; by_cases h_r1 : r1 = 20 <;> [
+      skip ; by_cases h_r1 : r1 = 21 <;> [
+      skip ; by_cases h_r1 : r1 = 22 <;> [
+      skip ; by_cases h_r1 : r1 = 23 <;> [
+      skip ; by_cases h_r1 : r1 = 24 <;> [
+      skip ; by_cases h_r1 : r1 = 25 <;> [
+      skip ; by_cases h_r1 : r1 = 26 <;> [
+      skip ; by_cases h_r1 : r1 = 27 <;> [
+      skip ; by_cases h_r1 : r1 = 28 <;> [
+      skip ; by_cases h_r1 : r1 = 29 <;> [
+      skip ; by_cases h_r1 : r1 = 30 <;> [
+      skip ; by_cases h_r1 : r1 = 31 <;> [
+        skip; (exfalso; grind)
+      ]
+    ]]]]]]]]]]]]]]]]]]]]]]]]]]]]]]
+    all_goals {
+      simp [
+        h_r1, LeanRV32D.Functions.rX_bits, LeanRV32D.Functions.rX,
+        Sail.readReg, PreSail.readReg, write_reg_state,
+        LeanRV32D.Functions.regval_from_reg
+      ] at ⊢ h_r1_val
+      unfold get instMonadStateOfMonadStateOf getThe MonadStateOf.get EStateM.instMonadStateOf EStateM.get at ⊢ h_r1_val
+      dsimp at ⊢ h_r1_val
+      have :
+        (state.regs.insert Register.nextPC (Sail.BitVec.addInt pc 4)).get? (bitvec_to_reg r1) =
+        state.regs.get? (bitvec_to_reg r1)
+      := by rewrite [h_r1]; simp [bitvec_to_reg]; grind
+      rewrite [h_r1] at this
+      simp [bitvec_to_reg] at this
+      simp [this]
+      have : ∃ x_val, state.regs.get? (bitvec_to_reg r1) = .some x_val := by
+        by_cases h_contr : ∃ x_val, state.regs.get? (bitvec_to_reg r1) = .some x_val
+        . assumption
+        . rewrite [h_r1] at h_contr
+          simp [bitvec_to_reg] at h_contr
+          apply Option.eq_none_iff_forall_ne_some.mpr at h_contr
+          simp [h_contr] at h_r1_val
+      rewrite [h_r1] at this
+      simp [bitvec_to_reg] at this
+      obtain ⟨x, h_x⟩ := this
+      simp [h_x] at ⊢ h_r1_val
+      exact h_r1_val
+    }
+
+  lemma mstatus_of_write_state
+    {mstatus : BitVec 64}
+    (pc : BitVec 32)
+    (h_mstatus : Sail.readReg Register.mstatus state = EStateM.Result.ok mstatus state)
+  :
+    Sail.readReg Register.mstatus (write_reg_state state Register.nextPC (Sail.BitVec.addInt pc 4)) =
+    EStateM.Result.ok mstatus (write_reg_state state Register.nextPC (Sail.BitVec.addInt pc 4))
+  := by
+    simp [
+      Sail.readReg, PreSail.readReg, write_reg_state
+    ] at ⊢ h_mstatus
+    unfold get instMonadStateOfMonadStateOf getThe MonadStateOf.get EStateM.instMonadStateOf EStateM.get at ⊢ h_mstatus
+    dsimp at ⊢ h_mstatus
+    have :
+      (state.regs.insert Register.nextPC (Sail.BitVec.addInt pc 4)).get? Register.mstatus =
+      state.regs.get? Register.mstatus
+    := by grind
+    simp [this]
+    rcases h: state.regs.get? Register.mstatus
+    . simp [h] at h_mstatus
+    . simp [h] at ⊢ h_mstatus
+      exact h_mstatus
+
+  lemma cur_privilege_of_write_state
+    {cur_privilege : Privilege}
+    (pc : BitVec 32)
+    (h_cur_privilege : Sail.readReg Register.cur_privilege state = EStateM.Result.ok cur_privilege state)
+  :
+    Sail.readReg Register.cur_privilege (write_reg_state state Register.nextPC (Sail.BitVec.addInt pc 4)) =
+    EStateM.Result.ok cur_privilege (write_reg_state state Register.nextPC (Sail.BitVec.addInt pc 4))
+  := by
+    simp [
+      Sail.readReg, PreSail.readReg, write_reg_state
+    ] at ⊢ h_cur_privilege
+    unfold get instMonadStateOfMonadStateOf getThe MonadStateOf.get EStateM.instMonadStateOf EStateM.get at ⊢ h_cur_privilege
+    dsimp at ⊢ h_cur_privilege
+    have :
+      (state.regs.insert Register.nextPC (Sail.BitVec.addInt pc 4)).get? Register.cur_privilege =
+      state.regs.get? Register.cur_privilege
+    := by grind
+    simp [this]
+    rcases h: state.regs.get? Register.cur_privilege
+    . simp [h] at h_cur_privilege
+    . simp [h] at ⊢ h_cur_privilege
+      exact h_cur_privilege
+
+  lemma clint_base_of_write_state
+    {clint_base : BitVec 34}
+    (pc : BitVec 32)
+    (h_clint_base : Sail.readReg Register.plat_clint_base state = EStateM.Result.ok clint_base state)
+  :
+    Sail.readReg Register.plat_clint_base (write_reg_state state Register.nextPC (Sail.BitVec.addInt pc 4)) =
+    EStateM.Result.ok clint_base (write_reg_state state Register.nextPC (Sail.BitVec.addInt pc 4))
+  := by
+    simp [
+      Sail.readReg, PreSail.readReg, write_reg_state
+    ] at ⊢ h_clint_base
+    unfold get instMonadStateOfMonadStateOf getThe MonadStateOf.get EStateM.instMonadStateOf EStateM.get at ⊢ h_clint_base
+    dsimp at ⊢ h_clint_base
+    have :
+      (state.regs.insert Register.nextPC (Sail.BitVec.addInt pc 4)).get? Register.plat_clint_base =
+      state.regs.get? Register.plat_clint_base
+    := by grind
+    simp [this]
+    rcases h: state.regs.get? Register.plat_clint_base
+    . simp [h] at h_clint_base
+    . simp [h] at ⊢ h_clint_base
+      exact h_clint_base
+
+  lemma clint_size_of_write_state
+    {clint_size : BitVec 34}
+    (pc : BitVec 32)
+    (h_clint_size : Sail.readReg Register.plat_clint_size state = EStateM.Result.ok clint_size state)
+  :
+    Sail.readReg Register.plat_clint_size (write_reg_state state Register.nextPC (Sail.BitVec.addInt pc 4)) =
+    EStateM.Result.ok clint_size (write_reg_state state Register.nextPC (Sail.BitVec.addInt pc 4))
+  := by
+    simp [
+      Sail.readReg, PreSail.readReg, write_reg_state
+    ] at ⊢ h_clint_size
+    unfold get instMonadStateOfMonadStateOf getThe MonadStateOf.get EStateM.instMonadStateOf EStateM.get at ⊢ h_clint_size
+    dsimp at ⊢ h_clint_size
+    have :
+      (state.regs.insert Register.nextPC (Sail.BitVec.addInt pc 4)).get? Register.plat_clint_size =
+      state.regs.get? Register.plat_clint_size
+    := by grind
+    simp [this]
+    rcases h: state.regs.get? Register.plat_clint_size
+    . simp [h] at h_clint_size
+    . simp [h] at ⊢ h_clint_size
+      exact h_clint_size
+
+  lemma ram_base_of_write_state
+    {ram_base : BitVec 34}
+    (pc : BitVec 32)
+    (h_ram_base : Sail.readReg Register.plat_ram_base state = EStateM.Result.ok ram_base state)
+  :
+    Sail.readReg Register.plat_ram_base (write_reg_state state Register.nextPC (Sail.BitVec.addInt pc 4)) =
+    EStateM.Result.ok ram_base (write_reg_state state Register.nextPC (Sail.BitVec.addInt pc 4))
+  := by
+    simp [
+      Sail.readReg, PreSail.readReg, write_reg_state
+    ] at ⊢ h_ram_base
+    unfold get instMonadStateOfMonadStateOf getThe MonadStateOf.get EStateM.instMonadStateOf EStateM.get at ⊢ h_ram_base
+    dsimp at ⊢ h_ram_base
+    have :
+      (state.regs.insert Register.nextPC (Sail.BitVec.addInt pc 4)).get? Register.plat_ram_base =
+      state.regs.get? Register.plat_ram_base
+    := by grind
+    simp [this]
+    rcases h: state.regs.get? Register.plat_ram_base
+    . simp [h] at h_ram_base
+    . simp [h] at ⊢ h_ram_base
+      exact h_ram_base
+
+  lemma ram_size_of_write_state
+    {ram_size : BitVec 34}
+    (pc : BitVec 32)
+    (h_ram_size : Sail.readReg Register.plat_ram_size state = EStateM.Result.ok ram_size state)
+  :
+    Sail.readReg Register.plat_ram_size (write_reg_state state Register.nextPC (Sail.BitVec.addInt pc 4)) =
+    EStateM.Result.ok ram_size (write_reg_state state Register.nextPC (Sail.BitVec.addInt pc 4))
+  := by
+    simp [
+      Sail.readReg, PreSail.readReg, write_reg_state
+    ] at ⊢ h_ram_size
+    unfold get instMonadStateOfMonadStateOf getThe MonadStateOf.get EStateM.instMonadStateOf EStateM.get at ⊢ h_ram_size
+    dsimp at ⊢ h_ram_size
+    have :
+      (state.regs.insert Register.nextPC (Sail.BitVec.addInt pc 4)).get? Register.plat_ram_size =
+      state.regs.get? Register.plat_ram_size
+    := by grind
+    simp [this]
+    rcases h: state.regs.get? Register.plat_ram_size
+    . simp [h] at h_ram_size
+    . simp [h] at ⊢ h_ram_size
+      exact h_ram_size
+
+  lemma rom_base_of_write_state
+    {rom_base : BitVec 34}
+    (pc : BitVec 32)
+    (h_rom_base : Sail.readReg Register.plat_rom_base state = EStateM.Result.ok rom_base state)
+  :
+    Sail.readReg Register.plat_rom_base (write_reg_state state Register.nextPC (Sail.BitVec.addInt pc 4)) =
+    EStateM.Result.ok rom_base (write_reg_state state Register.nextPC (Sail.BitVec.addInt pc 4))
+  := by
+    simp [
+      Sail.readReg, PreSail.readReg, write_reg_state
+    ] at ⊢ h_rom_base
+    unfold get instMonadStateOfMonadStateOf getThe MonadStateOf.get EStateM.instMonadStateOf EStateM.get at ⊢ h_rom_base
+    dsimp at ⊢ h_rom_base
+    have :
+      (state.regs.insert Register.nextPC (Sail.BitVec.addInt pc 4)).get? Register.plat_rom_base =
+      state.regs.get? Register.plat_rom_base
+    := by grind
+    simp [this]
+    rcases h: state.regs.get? Register.plat_rom_base
+    . simp [h] at h_rom_base
+    . simp [h] at ⊢ h_rom_base
+      exact h_rom_base
+
+  lemma rom_size_of_write_state
+    {rom_size : BitVec 34}
+    (pc : BitVec 32)
+    (h_rom_size : Sail.readReg Register.plat_rom_size state = EStateM.Result.ok rom_size state)
+  :
+    Sail.readReg Register.plat_rom_size (write_reg_state state Register.nextPC (Sail.BitVec.addInt pc 4)) =
+    EStateM.Result.ok rom_size (write_reg_state state Register.nextPC (Sail.BitVec.addInt pc 4))
+  := by
+    simp [
+      Sail.readReg, PreSail.readReg, write_reg_state
+    ] at ⊢ h_rom_size
+    unfold get instMonadStateOfMonadStateOf getThe MonadStateOf.get EStateM.instMonadStateOf EStateM.get at ⊢ h_rom_size
+    dsimp at ⊢ h_rom_size
+    have :
+      (state.regs.insert Register.nextPC (Sail.BitVec.addInt pc 4)).get? Register.plat_rom_size =
+      state.regs.get? Register.plat_rom_size
+    := by grind
+    simp [this]
+    rcases h: state.regs.get? Register.plat_rom_size
+    . simp [h] at h_rom_size
+    . simp [h] at ⊢ h_rom_size
+      exact h_rom_size
+
+  lemma htif_tohost_base_of_write_state
+    {htif_tohost_base : Option (BitVec 34)}
+    (pc : BitVec 32)
+    (h_htif_tohost_base : Sail.readReg Register.htif_tohost_base state = EStateM.Result.ok htif_tohost_base state)
+  :
+    Sail.readReg Register.htif_tohost_base (write_reg_state state Register.nextPC (Sail.BitVec.addInt pc 4)) =
+    EStateM.Result.ok htif_tohost_base (write_reg_state state Register.nextPC (Sail.BitVec.addInt pc 4))
+  := by
+    simp [
+      Sail.readReg, PreSail.readReg, write_reg_state
+    ] at ⊢ h_htif_tohost_base
+    unfold get instMonadStateOfMonadStateOf getThe MonadStateOf.get EStateM.instMonadStateOf EStateM.get at ⊢ h_htif_tohost_base
+    dsimp at ⊢ h_htif_tohost_base
+    have :
+      (state.regs.insert Register.nextPC (Sail.BitVec.addInt pc 4)).get? Register.htif_tohost_base =
+      state.regs.get? Register.htif_tohost_base
+    := by grind
+    simp [this]
+    rcases h: state.regs.get? Register.htif_tohost_base
+    . simp [h] at h_htif_tohost_base
+    . simp [h] at ⊢ h_htif_tohost_base
+      exact h_htif_tohost_base
+
+  set_option maxHeartbeats 0 in
   lemma execute_LOAD_lw_pure_equiv
     (lw_input : LwInput)
     (h_assumptions : lw_state_assumptions lw_input state)
@@ -174,7 +465,6 @@ namespace PureSpec
     rewrite [h_plat_rom_base_val] at h_plat_rom_base
     rewrite [h_htif_tohost_base_val] at h_htif_tohost_base
 
-
     simp [
       readReg_state h_pc,
       writeReg_state_success,
@@ -186,103 +476,19 @@ namespace PureSpec
     ]
     simp
 
-    set state' := (write_reg_state state Register.nextPC (Sail.BitVec.addInt lw_input.PC 4)) with h_state'
-
-    replace h_r1_val : LeanRV32D.Functions.rX_bits (regidx.Regidx lw_input.r1) state' = EStateM.Result.ok lw_input.r1_val state' := by
-      clear *- h_r1_val h_state'
-      rewrite [h_state']
-      by_cases h_r1: lw_input.r1 = 0
-      . simp [
-         h_r1, LeanRV32D.Functions.rX_bits, LeanRV32D.Functions.rX
-        ] at ⊢ h_r1_val
-        exact h_r1_val
-      by_cases h_r1 : lw_input.r1 = 1 <;> [
-        skip ; by_cases h_r1 : lw_input.r1 = 2 <;> [
-        skip ; by_cases h_r1 : lw_input.r1 = 3 <;> [
-        skip ; by_cases h_r1 : lw_input.r1 = 4 <;> [
-        skip ; by_cases h_r1 : lw_input.r1 = 5 <;> [
-        skip ; by_cases h_r1 : lw_input.r1 = 6 <;> [
-        skip ; by_cases h_r1 : lw_input.r1 = 7 <;> [
-        skip ; by_cases h_r1 : lw_input.r1 = 8 <;> [
-        skip ; by_cases h_r1 : lw_input.r1 = 9 <;> [
-        skip ; by_cases h_r1 : lw_input.r1 = 10 <;> [
-        skip ; by_cases h_r1 : lw_input.r1 = 11 <;> [
-        skip ; by_cases h_r1 : lw_input.r1 = 12 <;> [
-        skip ; by_cases h_r1 : lw_input.r1 = 13 <;> [
-        skip ; by_cases h_r1 : lw_input.r1 = 14 <;> [
-        skip ; by_cases h_r1 : lw_input.r1 = 15 <;> [
-        skip ; by_cases h_r1 : lw_input.r1 = 16 <;> [
-        skip ; by_cases h_r1 : lw_input.r1 = 17 <;> [
-        skip ; by_cases h_r1 : lw_input.r1 = 18 <;> [
-        skip ; by_cases h_r1 : lw_input.r1 = 19 <;> [
-        skip ; by_cases h_r1 : lw_input.r1 = 20 <;> [
-        skip ; by_cases h_r1 : lw_input.r1 = 21 <;> [
-        skip ; by_cases h_r1 : lw_input.r1 = 22 <;> [
-        skip ; by_cases h_r1 : lw_input.r1 = 23 <;> [
-        skip ; by_cases h_r1 : lw_input.r1 = 24 <;> [
-        skip ; by_cases h_r1 : lw_input.r1 = 25 <;> [
-        skip ; by_cases h_r1 : lw_input.r1 = 26 <;> [
-        skip ; by_cases h_r1 : lw_input.r1 = 27 <;> [
-        skip ; by_cases h_r1 : lw_input.r1 = 28 <;> [
-        skip ; by_cases h_r1 : lw_input.r1 = 29 <;> [
-        skip ; by_cases h_r1 : lw_input.r1 = 30 <;> [
-        skip ; by_cases h_r1 : lw_input.r1 = 31 <;> [
-          skip; (exfalso; grind)
-        ]
-      ]]]]]]]]]]]]]]]]]]]]]]]]]]]]]]
-      all_goals {
-        simp [
-          h_r1, LeanRV32D.Functions.rX_bits, LeanRV32D.Functions.rX,
-          Sail.readReg, PreSail.readReg, write_reg_state,
-          LeanRV32D.Functions.regval_from_reg
-        ] at ⊢ h_r1_val
-        unfold get instMonadStateOfMonadStateOf getThe MonadStateOf.get EStateM.instMonadStateOf EStateM.get at ⊢ h_r1_val
-        dsimp at ⊢ h_r1_val
-        have :
-          (state.regs.insert Register.nextPC (Sail.BitVec.addInt lw_input.PC 4)).get? (bitvec_to_reg lw_input.r1) =
-          state.regs.get? (bitvec_to_reg lw_input.r1)
-        := by rewrite [h_r1]; simp [bitvec_to_reg]; grind
-        rewrite [h_r1] at this
-        simp [bitvec_to_reg] at this
-        simp [this]
-        have : ∃ x_val, state.regs.get? (bitvec_to_reg lw_input.r1) = .some x_val := by
-          by_cases h_contr : ∃ x_val, state.regs.get? (bitvec_to_reg lw_input.r1) = .some x_val
-          . assumption
-          . rewrite [h_r1] at h_contr
-            simp [bitvec_to_reg] at h_contr
-            apply Option.eq_none_iff_forall_ne_some.mpr at h_contr
-            simp [h_contr] at h_r1_val
-            done
-        rewrite [h_r1] at this
-        simp [bitvec_to_reg] at this
-        obtain ⟨x, h_x⟩ := this
-        simp [h_x] at ⊢ h_r1_val
-        exact h_r1_val
-      }
-
-    replace h_mstatus :
-      Sail.readReg Register.mstatus state' =
-      EStateM.Result.ok lw_input.mstatus state'
-    := by
-      rewrite [h_state']
-      clear *-h_mstatus
-      simp [
-        Sail.readReg, PreSail.readReg, write_reg_state
-      ] at ⊢ h_mstatus
-      unfold get instMonadStateOfMonadStateOf getThe MonadStateOf.get EStateM.instMonadStateOf EStateM.get at ⊢ h_mstatus
-      dsimp at ⊢ h_mstatus
-      have :
-        (state.regs.insert Register.nextPC (Sail.BitVec.addInt lw_input.PC 4)).get? Register.mstatus =
-        state.regs.get? Register.mstatus
-      := by grind
-      simp [this, h_mstatus]
-      done
-
-
-
+    replace h_r1_val := r1_of_write_state lw_input.PC h_r1_val
+    replace h_mstatus := mstatus_of_write_state lw_input.PC h_mstatus
+    replace h_cur_privilege := cur_privilege_of_write_state lw_input.PC h_cur_privilege
+    replace h_clint_base := clint_base_of_write_state lw_input.PC h_clint_base
+    replace h_clint_size := clint_size_of_write_state lw_input.PC h_clint_size
+    replace h_plat_ram_base := ram_base_of_write_state lw_input.PC h_plat_ram_base
+    replace h_plat_ram_size := ram_size_of_write_state lw_input.PC h_plat_ram_size
+    replace h_plat_rom_base := rom_base_of_write_state lw_input.PC h_plat_rom_base
+    replace h_plat_rom_size := rom_size_of_write_state lw_input.PC h_plat_rom_size
+    replace h_htif_tohost_base := htif_tohost_base_of_write_state lw_input.PC h_htif_tohost_base
 
     have h_execute_load := Local.execute_LOAD_simplified
-      state'
+      (write_reg_state state Register.nextPC (Sail.BitVec.addInt lw_input.PC 4))
       (regidx.Regidx lw_input.rd)
       lw_input.data0
       lw_input.data1
@@ -290,90 +496,48 @@ namespace PureSpec
       lw_input.data3
       h_aligned
       h_r1_val
-      -- h_mstatus
-      -- h_cur_privilege
-      -- h_clint_base
-      -- h_clint_size
-      -- h_plat_ram_base
-      -- h_plat_rom_base
-      -- h_plat_ram_size
-      -- h_plat_rom_size
-      -- h_htif_tohost_base
-      -- h_mstatus_val
-      -- h_does_fit
-      -- h_mem_0
-      -- h_mem_1
-      -- h_mem_2
-      -- h_mem_3
+      h_mstatus
+      h_cur_privilege
+      h_clint_base
+      h_clint_size
+      h_plat_ram_base
+      h_plat_rom_base
+      h_plat_ram_size
+      h_plat_rom_size
+      h_htif_tohost_base
+      h_mstatus_val
+      h_does_fit
+      h_mem_0 -- this works because write_reg_state doesn't affect state.mem
+      h_mem_1
+      h_mem_2
+      h_mem_3
 
     rewrite [
-      Local.execute_LOAD_equiv,
       h_execute_load
     ]
 
-
-
-    unfold bind Monad.toBind EStateM.instMonad
-    dsimp
-    unfold EStateM.bind
-    dsimp
-
     simp [
-      readReg_state h_input_pc,
-      writeReg_state_success,
-      ←Local.execute_equiv,
-      Local.execute.eq_def
+      execute_LOAD_lw_pure
     ]
-
-    have (x : BitVec 32) : Sail.BitVec.addInt x 4 = x + 4 := rfl
-    simp [this]
-
-    have := Local.execute_LOAD_simplified
-      lw_input.data0
-      lw_input.data1
-      lw_input.data2
-      lw_input.data3
-
-
-    simp [
-      Local.execute_LOAD_simplified
-    ]
-
-    simp [
-      ←Local.execute_RTYPE_equiv,
-      Local.execute_RTYPE.eq_def,
-      bind, EStateM.instMonad, EStateM.bind
-    ]
-
-    rewrite [rX_read_xreg_equiv _ r1 (regidx_to_fin r1) (by simp [regidx_to_fin])]
-    rewrite [read_xreg_write_reg_state_nextPC _ h_input_r1]
-    simp
-    rewrite [rX_read_xreg_equiv _ r2 (regidx_to_fin r2) (by simp [regidx_to_fin])]
-    rewrite [read_xreg_write_reg_state_nextPC _ h_input_r2]
-    simp [EStateM.pure]
-
-    simp [execute_RTYPE_add_pure]
-
-    obtain ⟨rd⟩ := rd
-    by_cases h_zero: rd = 0
-    . rewrite [h_zero, wX_write_xreg_0_equiv]
-      simp
-      rewrite [dite_cond_eq_true]
-      . simp
-      . simp [h_input_rd, h_zero, regidx_to_fin]
-    . have h_inc := regidx_non_zero h_zero
-      apply Finset.mem_Icc.mp at h_inc
-      obtain ⟨h_low, h_high⟩ := h_inc
+    split_ifs with h_rd
+    . simp [
+        LeanRV32D.Functions.wX_bits,
+        LeanRV32D.Functions.wX,
+        h_rd,
+        Sail.BitVec.addInt
+      ]
+    . simp [Sail.BitVec.addInt]
       rewrite [
         wX_write_xreg_equiv _ _
-          (regidx.Regidx rd)
-          ⟨(regidx_to_fin (regidx.Regidx rd)).val, Finset.mem_Icc.mpr ⟨h_low, h_high⟩⟩
-          (by simp [regidx_to_fin])
+          (regidx.Regidx lw_input.rd)
+          ⟨lw_input.rd.toNat, range lw_input.rd h_rd⟩
       ]
-      simp [regidx_to_fin]
-      rewrite [dite_cond_eq_false]
-      . simp [h_input_rd, regidx_to_fin]
-      . simp [regidx_to_fin] at *
-        omega
+      . obtain s | s := write_xreg
+          ⟨lw_input.rd.toNat, _⟩
+          (lw_input.data3 ++ lw_input.data2 ++ lw_input.data1 ++ lw_input.data0)
+          (write_reg_state state Register.nextPC (lw_input.PC + 4#32))
+        . simp
+        . simp
+      . simp
 
 end PureSpec
